iris/KernelDecode09.v
@@ -486,6 +486,11 @@ Lemma kd_05505163 s : register_lookup misa (sregs s) = MISA_C -> cfg_ok s ->
   = Some (BTYPE (mword_of_int 66 : mword 13, Regidx (mword_of_int 21), zreg, BGE), s).
 Proof. decode_bridge_ms. Qed.
 
+Lemma kd_0559f363 s : register_lookup misa (sregs s) = MISA_C -> cfg_ok s ->
+  exec (ext_decode (mword_of_int 0x0559f363 : mword 32) : M instruction) s
+  = Some (BTYPE (mword_of_int 70 : mword 13, Regidx (mword_of_int 21), Regidx (mword_of_int 19), BGEU), s).
+Proof. decode_bridge_ms. Qed.
+
 Lemma kd_05893683 s : register_lookup misa (sregs s) = MISA_C -> cfg_ok s ->
   exec (ext_decode (mword_of_int 0x05893683 : mword 32) : M instruction) s
   = Some (LOAD (mword_of_int 88 : mword 12, Regidx (mword_of_int 18), Regidx (mword_of_int 13), false, 8), s).
