iris/KernelDecode11.v
@@ -496,6 +496,11 @@ Lemma kd_080000ef s : register_lookup misa (sregs s) = MISA_C -> cfg_ok s ->
   = Some (JAL (mword_of_int 128 : mword 21, Regidx (mword_of_int 1)), s).
 Proof. decode_bridge_ms. Qed.
 
+Lemma kd_080a8b63 s : register_lookup misa (sregs s) = MISA_C -> cfg_ok s ->
+  exec (ext_decode (mword_of_int 0x080a8b63 : mword 32) : M instruction) s
+  = Some (BTYPE (mword_of_int 150 : mword 13, zreg, Regidx (mword_of_int 21), BEQ), s).
+Proof. decode_bridge_ms. Qed.
+
 Lemma kd_0ef77b63 s : register_lookup misa (sregs s) = MISA_C -> cfg_ok s ->
   exec (ext_decode (mword_of_int 0x0ef77b63 : mword 32) : M instruction) s
   = Some (BTYPE (mword_of_int 246 : mword 13, Regidx (mword_of_int 15), Regidx (mword_of_int 14), BGEU), s).
