iris/KernelDecode13.v
@@ -466,6 +466,11 @@ Lemma kd_0007a023 s : register_lookup misa (sregs s) = MISA_C -> cfg_ok s ->
   = Some (STORE (mword_of_int 0 : mword 12, zreg, Regidx (mword_of_int 15), 4), s).
 Proof. decode_bridge_ms. Qed.
 
+Lemma kd_000b2503 s : register_lookup misa (sregs s) = MISA_C -> cfg_ok s ->
+  exec (ext_decode (mword_of_int 0x000b2503 : mword 32) : M instruction) s
+  = Some (LOAD (mword_of_int 0 : mword 12, Regidx (mword_of_int 22), Regidx (mword_of_int 10), false, 4), s).
+Proof. decode_bridge_ms. Qed.
+
 Lemma kd_000f4737 s : register_lookup misa (sregs s) = MISA_C -> cfg_ok s ->
   exec (ext_decode (mword_of_int 0x000f4737 : mword 32) : M instruction) s
   = Some (UTYPE (mword_of_int 244 : mword 20, Regidx (mword_of_int 14), LUI), s).
@@ -586,9 +591,19 @@ Lemma kd_05848513 s : register_lookup misa (sregs s) = MISA_C -> cfg_ok s ->
   = Some (ITYPE (mword_of_int 88 : mword 12, Regidx (mword_of_int 9), Regidx (mword_of_int 10), ADDI), s).
 Proof. decode_bridge_ms. Qed.
 
+Lemma kd_05850363 s : register_lookup misa (sregs s) = MISA_C -> cfg_ok s ->
+  exec (ext_decode (mword_of_int 0x05850363 : mword 32) : M instruction) s
+  = Some (BTYPE (mword_of_int 70 : mword 13, Regidx (mword_of_int 24), Regidx (mword_of_int 10), BEQ), s).
+Proof. decode_bridge_ms. Qed.
+
 Lemma kd_05850663 s : register_lookup misa (sregs s) = MISA_C -> cfg_ok s ->
   exec (ext_decode (mword_of_int 0x05850663 : mword 32) : M instruction) s
   = Some (BTYPE (mword_of_int 76 : mword 13, Regidx (mword_of_int 24), Regidx (mword_of_int 10), BEQ), s).
+Proof. decode_bridge_ms. Qed.
+
+Lemma kd_05890613 s : register_lookup misa (sregs s) = MISA_C -> cfg_ok s ->
+  exec (ext_decode (mword_of_int 0x05890613 : mword 32) : M instruction) s
+  = Some (ITYPE (mword_of_int 88 : mword 12, Regidx (mword_of_int 18), Regidx (mword_of_int 12), ADDI), s).
 Proof. decode_bridge_ms. Qed.
 
 Lemma kd_07300793 s : register_lookup misa (sregs s) = MISA_C -> cfg_ok s ->
